src/simulation_steps/IssueReservedRelPlainStep.v
@@ -154,7 +154,6 @@ Proof using WF CON.
 
   assert (R r /\ W w) as [RREAD WWRITE].
   { apply (wf_rmwD WF) in RMW.
-    hahn_rewrite (R_ex_in_R) in RMW.
     apply seq_eqv_l in RMW; destruct RMW as [WW RMW].
     apply seq_eqv_r in RMW; desf. }
 
